Makefile
@@ -110,7 +110,8 @@ CFRONTEND=Ctypes.v Cop.v Csyntax.v Csem.v Ctyping.v Cstrategy.v Cexec.v \
   Clight.v ClightBigstep.v SimplLocals.v SimplLocalsproof.v \
   Cshmgen.v Cshmgenproof.v \
   Csharpminor.v Cminorgen.v Cminorgenproof.v \
-  Maple.v Mapletypes.v MapleOp.v MapleExec.v
+  Maple.v Mapletypes.v MapleOp.v MapleExec.v MapleDenotation.v\
+  ITree.v
 
 # Parser
 
